theories/iris.v
@@ -784,7 +784,7 @@ Instance heapG_irisG `{!hsG Σ, !locG Σ, !wfuncG Σ, !wtabG Σ, !wmemG Σ, !wgl
       (gen_heap_interp (gmap_of_list locs)) ∗
       (gen_heap_interp (gmap_of_list s.(s_funcs))) ∗
       (gen_heap_interp (gmap_of_table s.(s_tables))) ∗
-      (gen_heap_interp (gmap_of_mem s.(s_mems))) ∗
+      (gen_heap_interp (gmap_of_memory s.(s_mems))) ∗
       (gen_heap_interp (gmap_of_list s.(s_globals)))
     )%I;
   fork_post _ := True%I;
@@ -1869,262 +1869,6 @@ Qed.
       pure_reduce hs s locs (HE_wasm_table_create len) hs s' locs (HE_value (HV_wov (WOV_tableref (Mk_tableidx n))))
  *)
 
-Definition new_table_gmap_at_n (n: N) (len: nat) : gmap (N*N) funcelem:=
-  list_to_map (imap (fun i x => ((n, N.of_nat i), x)) (repeat None len)).
-
-Definition new_memory_gmap_at_n (n: N) (len: nat) : gmap (N*N) byte:=
-  list_to_map (imap (fun i x => ((n, N.of_nat i), x)) (repeat #00 len)).
-
-Lemma repeat_lookup {T: Type} (x: T) (n i: nat):
-  i < n <->
-  (repeat x n) !! i = Some x.
-Proof.
-  split. 
-  - move : n.
-    induction i; move => n HLen; destruct n => //=; try lia.
-    apply IHi.
-    lia.
-  - move => Hlookup.
-    apply lookup_lt_Some in Hlookup.
-    by rewrite repeat_length in Hlookup.
-Qed.
-
-Lemma new_table_gmap_at_n_lookup n i len:
-  (i<len)%N ->
-  new_table_gmap_at_n n (N.to_nat len) !! (n, i) = Some None.
-Proof.
-  move => HLen.
-  unfold new_table_gmap_at_n.
-  apply elem_of_list_to_map; resolve_finmap.
-  - apply Nat2N.inj in H0. subst.
-    rewrite Helem0 in Helem.
-    by inversion Helem.
-  - apply nodup_imap_inj1.
-    move => n1 n2 t1 t2 Heq.
-    inversion Heq.
-    by apply Nat2N.inj in H0.
-  - apply elem_of_lookup_imap.
-    exists (N.to_nat i), None.
-    split.
-    + repeat f_equal.
-      lia.
-    + apply repeat_lookup.
-      lia.
-Qed.
-      
-Lemma new_table_gmap_at_n_lookup_None n i len:
-  (i>=len)%N ->
-  new_table_gmap_at_n n (N.to_nat len) !! (n, i) = None.
-Proof.
-  move => HLen.
-  unfold new_table_gmap_at_n.
-  apply not_elem_of_list_to_map. move => HContra. resolve_finmap. subst => //=.
-  inversion Heq; subst; clear Heq.
-  apply lookup_lt_Some in Helem0.
-  rewrite repeat_length in Helem0.
-  lia.
-Qed.
-  
-Lemma new_table_gmap_at_n_lookup_None2 n m i len:
-  n <> m ->
-  new_table_gmap_at_n n (N.to_nat len) !! (m, i) = None.
-Proof.
-  move => Hneq.
-  unfold new_table_gmap_at_n.
-  apply not_elem_of_list_to_map. move => HContra. resolve_finmap. subst => //=.
-  by inversion Heq.
-Qed.
-  
-Lemma gmap_of_table_append_disjoint tab len:
-  new_table_gmap_at_n (N.of_nat (length tab)) (N.to_nat len) ##ₘ gmap_of_table tab.
-Proof.
-  apply map_disjoint_spec.
-  move => [n i] f1 f2 H1 H2.
-  unfold new_table_gmap_at_n in H1.
-  resolve_finmap.
-  - unfold gmap_of_table in H2.
-    rewrite gmap_of_list_2d_lookup in H2.
-    clear Helem.
-    rewrite Nat2N.id in H2.
-    destruct (_ !! length _ ) eqn: HContra => //. clear H2.
-    assert (Some l = None) => //.
-    rewrite - HContra. clear HContra.
-    apply lookup_ge_None.
-    rewrite fmap_length.
-    lia.
-  - apply Nat2N.inj in H1. subst.
-    rewrite Helem0 in Helem.
-    by inversion Helem.
-  - apply nodup_imap_inj1.
-    move => n1 n2 t1 t2 Heq.
-    inversion Heq.
-    by apply Nat2N.inj in H1.
-Qed.
-
-Lemma gmap_of_memory_append_disjoint mem len:
-  new_memory_gmap_at_n (N.of_nat (length mem)) (N.to_nat len) ##ₘ gmap_of_mem mem.
-Proof.
-  apply map_disjoint_spec.
-  move => [n i] f1 f2 H1 H2.
-  unfold new_memory_gmap_at_n in H1.
-  resolve_finmap.
-  - unfold gmap_of_mem in H2.
-    rewrite gmap_of_list_2d_lookup in H2.
-    clear Helem.
-    rewrite Nat2N.id in H2.
-    destruct (_ !! length _ ) eqn: HContra => //. clear H2.
-    assert (Some l = None) => //.
-    rewrite - HContra. clear HContra.
-    apply lookup_ge_None.
-    rewrite fmap_length.
-    lia.
-  - apply Nat2N.inj in H1. subst.
-    rewrite Helem0 in Helem.
-    by inversion Helem.
-  - apply nodup_imap_inj1.
-    move => n1 n2 t1 t2 Heq.
-    inversion Heq.
-    by apply Nat2N.inj in H1.
-Qed.
-    
-Lemma gmap_of_table_append l len:
-  gmap_of_table (l ++ [::create_table len]) =
-  new_table_gmap_at_n (N.of_nat (length l)) (N.to_nat len) ∪ gmap_of_table l.
-Proof.
-  apply map_eq.
-  move => [n i].
-  unfold gmap_of_table.
-  remember_lookup; rewrite gmap_of_list_2d_lookup in Hlookup.
-  destruct lookup_res => //=.
-  - destruct (_ !! N.to_nat n) eqn:Hlookup2 => //.
-    assert (N.to_nat n <= length l) as Hlen.
-    {
-      apply lookup_lt_Some in Hlookup2.
-      rewrite fmap_length app_length in Hlookup2.
-      simpl in Hlookup2.
-      lia.
-    }
-    destruct (decide (N.to_nat n = length l)) => //.
-    + rewrite e in Hlookup2.
-      rewrite list_lookup_fmap in Hlookup2.
-      rewrite lookup_app_r in Hlookup2; last lia.
-      replace (length l - length l) with 0 in Hlookup2; last lia.
-      simpl in Hlookup2.
-      inversion Hlookup2; subst; clear Hlookup2.
-      assert (N.to_nat i < N.to_nat len).
-      { apply lookup_lt_Some in Hlookup.
-        by rewrite repeat_length in Hlookup.
-      }
-      apply elem_of_list_lookup_2 in Hlookup.
-      apply elem_of_list_In in Hlookup.
-      apply repeat_spec in Hlookup. subst.
-      symmetry.
-      apply lookup_union_Some_l.
-      rewrite - e.
-      rewrite N2Nat.id.
-      apply new_table_gmap_at_n_lookup.
-      lia.
-    + assert (N.to_nat n < length l) as Hlenlt; first lia.
-      symmetry.
-      apply lookup_union_Some_r; first by apply gmap_of_table_append_disjoint.
-      rewrite gmap_of_list_2d_lookup.
-      rewrite list_lookup_fmap in Hlookup2.
-      rewrite list_lookup_fmap.
-      rewrite lookup_app_l in Hlookup2; last lia.
-      by rewrite Hlookup2.
-  - destruct (_ !! N.to_nat n) eqn:Hlookup2 => //.
-    + assert (N.to_nat n <= length l) as Hlen.
-      {
-        apply lookup_lt_Some in Hlookup2.
-        rewrite fmap_length app_length in Hlookup2.
-        simpl in Hlookup2.
-        lia.
-      }
-      destruct (decide (N.to_nat n = length l)) => //.
-      * rewrite e in Hlookup2.
-        rewrite list_lookup_fmap in Hlookup2.
-        rewrite lookup_app_r in Hlookup2; last lia.
-        replace (length l - length l) with 0 in Hlookup2; last lia.
-        simpl in Hlookup2.
-        inversion Hlookup2; subst; clear Hlookup2.
-        assert (N.to_nat i >= N.to_nat len).
-        { apply lookup_ge_None in Hlookup.
-          by rewrite repeat_length in Hlookup.
-        }
-        symmetry.
-        apply lookup_union_None.
-        split.
-        -- rewrite - e.
-          rewrite N2Nat.id.
-          apply new_table_gmap_at_n_lookup_None.
-          lia.
-        -- rewrite gmap_of_list_2d_lookup.
-          rewrite list_lookup_fmap.
-          assert (N.to_nat n ≥ length l) as Hlen2; first lia.
-          apply lookup_ge_None in Hlen2.
-          by rewrite Hlen2.
-      * assert (N.to_nat n < length l) as Hlenlt; first lia.
-        symmetry.
-        apply lookup_union_None.
-        split.
-        -- rewrite new_table_gmap_at_n_lookup_None2 => //.
-          lia.
-        -- rewrite gmap_of_list_2d_lookup.
-          rewrite list_lookup_fmap in Hlookup2.
-          rewrite lookup_app_l in Hlookup2; last lia.
-          by rewrite list_lookup_fmap Hlookup2.
-    + clear Hlookup.
-      rewrite list_lookup_fmap in Hlookup2.
-      destruct (_ !! N.to_nat n) eqn:Hlookup => //.
-      clear Hlookup2.
-      apply lookup_ge_None in Hlookup.
-      rewrite app_length in Hlookup.
-      simpl in Hlookup.
-      symmetry.
-      apply lookup_union_None.
-      split.
-      * apply new_table_gmap_at_n_lookup_None2 => //.
-        lia.
-      * rewrite gmap_of_list_2d_lookup.
-        rewrite list_lookup_fmap.
-        assert (N.to_nat n >= length l) as Hlen; first lia.
-        apply lookup_ge_None in Hlen.
-        by rewrite Hlen.
-Qed.
-
-Lemma gmap_of_table_insert n i x l t:
-  l !! n = Some t ->
-  i < length t.(table_data) ->
-  <[(N.of_nat n,N.of_nat i) := x]> (gmap_of_table l) = gmap_of_table (<[n := {|table_data := (<[i := x]> t.(table_data)); table_max_opt := t.(table_max_opt)|}]> l).
-Proof.
-  move => HLookup HLen.
-  apply map_eq.
-  move => [m j].
-  unfold gmap_of_table.
-  remember_lookup. rewrite gmap_of_list_2d_lookup. symmetry.
-  destruct (decide ((N.of_nat n, N.of_nat i) = (m,j))).
-  - inversion e; subst; clear e.
-    repeat rewrite Nat2N.id.
-    rewrite lookup_insert.
-    rewrite list_lookup_fmap => //.
-    rewrite list_lookup_insert => /=; last by apply lookup_lt_Some in HLookup.
-    by rewrite list_lookup_insert.
-  - rewrite lookup_insert_ne in Hlookup => //.
-    rewrite list_lookup_fmap.
-    destruct (decide (n = N.to_nat m)); subst.
-    + rewrite list_lookup_insert => /=; last by apply lookup_lt_Some in HLookup.
-      destruct (decide (i = N.to_nat j)).
-      * exfalso. apply n0. subst.
-        by repeat rewrite N2Nat.id.
-      * rewrite list_lookup_insert_ne => //=.
-        rewrite gmap_of_list_2d_lookup.
-        rewrite list_lookup_fmap.
-        by rewrite HLookup.
-    + rewrite list_lookup_insert_ne => //=.
-      rewrite gmap_of_list_2d_lookup.
-      by rewrite list_lookup_fmap.
-Qed.
-      
 Lemma wp_table_create len s E:
   ⊢
   (WP HE_wasm_table_create len @ s; E
@@ -2161,7 +1905,8 @@ Proof.
     *)
     iMod (gen_heap_alloc_big with "Hwt") as "(Hwt & Hl & Hm)".
     {
-      instantiate (1 := new_table_gmap_at_n (N.of_nat (length ws.(s_tables))) (N.to_nat len)).
+      unfold gmap_of_table.
+      instantiate (1 := new_2d_gmap_at_n (N.of_nat (length ws.(s_tables))) (N.to_nat len) None).
       by apply gmap_of_table_append_disjoint.
     }
     iModIntro.
@@ -2173,15 +1918,16 @@ Proof.
       (* This is the correct usage of premises with big_sepM [∗ map] like this. Add a bit more
          comments in the future -- this will surely be forgotten in the future. *)
       iDestruct (big_sepM_lookup with "Hl") as "Hni" => //.
-      by apply new_table_gmap_at_n_lookup.
+      apply new_2d_gmap_at_n_lookup.
+      lia.
 Qed.
 
 Ltac simplify_lookup :=
   repeat match goal with
   | H: gmap_of_table _ !! _ = _ |- _ =>
        unfold gmap_of_table in H
-  | H: gmap_of_mem _ !! _ = _ |- _ =>
-       unfold gmap_of_mem in H
+  | H: gmap_of_memory _ !! _ = _ |- _ =>
+       unfold gmap_of_memory in H
   | H: gmap_of_list_2d _ !! _ = _ |- _ =>
        rewrite gmap_of_list_2d_lookup in H
   | H: gmap_of_list_lookup _ !! _ = _ |- _ =>
@@ -2238,8 +1984,8 @@ Proof.
     iMod (gen_heap_update with "Hwt Hfunc") as "[Hwt Hfunc]".
     iModIntro.
     iFrame.
-    rewrite - gmap_of_table_insert => //.
-    rewrite N2Nat.id.
+    erewrite gmap_of_table_insert => //; last by rewrite Nat2N.id.
+    rewrite Nat2N.id.
     iFrame.
     iSplitL => //.
     iApply ("HΦ" with "[Hfuncref Htableref Hfunc]").
@@ -2319,18 +2065,19 @@ Proof.
     inv_head_step.
     iMod (gen_heap_alloc_big with "Hwm") as "(Hwm & Hl & Hm)".
     {
-      instantiate (1 := new_memory_gmap_at_n (N.of_nat (length ws.(s_mems))) (N.to_nat sz)).
+      instantiate (1 := new_2d_gmap_at_n (N.of_nat (length ws.(s_mems))) (N.to_nat sz) #00).
       by apply gmap_of_memory_append_disjoint.
     }
     iModIntro.
     iFrame.
     iSplitL "Hwm".
-    + admit.
+    + by rewrite gmap_of_memory_append.
     + iSplit => //.
       iIntros (i) "%H".
       iDestruct (big_sepM_lookup with "Hl") as "Hni" => //.
-      admit.
-Admitted.
+      rewrite new_2d_gmap_at_n_lookup => //.
+      lia.
+Qed.
 (*  
   | pr_memory_set:
     forall hs s locs idm n id md' mn m m' s' b,
